nola/examples/logic/deriv.v
@@ -20,5 +20,6 @@ Notation "⟦ P ⟧" := ⟦ P ⟧(nderiv) : nola_scope.
 Notation "⟦ P ⟧ˢ" := ⟦ P ⟧ˢ(nderiv) : nola_scope.
 Notation inv_wsatd := (inv_wsat' nderiv).
 Notation na_inv_wsatd := (na_inv_wsat' nderiv).
+Notation borrow_wsatd W E := (borrow_wsat' nderiv W E).
 
 Implicit Type P : nPropL (;ᵞ).
